steel/Zeta.Steel.IArray.fst
@@ -1,0 +1,123 @@
+module Zeta.Steel.IArray
+
+module G = FStar.Ghost
+module ETbl = Steel.ST.EphemeralHashtbl
+
+let tbl #k #v #contents h vp = finalizer:ETbl.finalizer_t vp & ETbl.tbl h finalizer
+
+let repr_to_eht_repr (#k:eqtype) (#contents:Type0) (m:repr k contents)
+  : ETbl.repr k contents
+  = PartialMap.literal (fun x -> if m `Map.contains` x then Some (Map.sel m x) else None)
+
+let perm t m =
+  ETbl.tperm (dsnd t) (repr_to_eht_repr m) (PartialMap.empty _ _)
+
+let unpack_perm (#opened:_)
+  (#k:eqtype)
+  (#v #contents:Type0)
+  (#vp:EHT.vp_t k v contents)
+  (#h:EHT.hash_fn k)
+  (#m:G.erased (repr k contents))
+  (a:tbl h vp)
+  : STGhostT unit opened
+      (perm a m)
+      (fun _ -> ETbl.tperm (dsnd a) (repr_to_eht_repr m) (PartialMap.empty k v))
+  = rewrite (perm a m) _
+
+let pack_perm (#opened:_)
+  (#k:eqtype)
+  (#v #contents:Type0)
+  (#vp:EHT.vp_t k v contents)
+  (#h:EHT.hash_fn k)
+  (#finalizer:ETbl.finalizer_t vp)
+  (#e_m:ETbl.repr k contents)
+  (#e_borrows:PartialMap.t k v)
+  (e_a:ETbl.tbl h finalizer)
+  (a:tbl h vp)
+  (m:repr k contents)
+  : STGhost unit opened
+      (ETbl.tperm e_a e_m e_borrows)
+      (fun _ -> perm a m)
+      (requires
+        a == (| finalizer, e_a |) /\
+        PartialMap.equal e_m (repr_to_eht_repr m) /\
+        PartialMap.equal e_borrows (PartialMap.empty _ _))
+      (ensures fun _ -> True)
+  = rewrite _ (perm a m)
+
+let create #k #v #contents #vp h n finalize init =
+  let etbl = ETbl.create h finalize n in
+  let r = (| finalize, etbl |) in
+  pack_perm etbl r (Map.restrict Set.empty (Map.const #k #contents init));
+  return r
+
+let free a = ETbl.free (dsnd a)
+
+let put #k #v #contents #h #vp #m a i x c =
+  unpack_perm a;
+  ETbl.put (dsnd a) i x c;
+  pack_perm (dsnd a) a (Map.upd m i (G.reveal c))
+
+let remove #k #v #contents #h #vp #m a i =
+  unpack_perm a;
+  let b = ETbl.remove (dsnd a) i in
+  pack_perm (dsnd a) a m;
+  return b
+
+let etbl_with_key_post_to_with_key_post (#opened:_)
+  (#k:eqtype) (#v #contents:Type0) (#vp:ETbl.vp_t k v contents) (#h:ETbl.hash_fn k)
+  (#m:repr k contents)
+  (a:tbl h vp)
+  (i:k)
+  (#res:Type)
+  (f_pre:vprop)
+  (f_post:contents -> contents -> res -> vprop)
+  (r:ETbl.get_result k res)
+  : STGhostT unit opened
+      (ETbl.with_key_post (repr_to_eht_repr m) (PartialMap.empty _ _) (dsnd a) i f_pre f_post r)
+      (fun _ -> with_key_post m a i f_pre f_post r)
+  = let etbl_m = repr_to_eht_repr m in
+    match r, PartialMap.sel i etbl_m with
+    | ETbl.Present r0, Some c ->
+      rewrite
+        (ETbl.with_key_post _ _ _ _ _ _ _)
+        (exists_ (ETbl.with_key_post_present_predicate (repr_to_eht_repr m)
+                                                       (PartialMap.empty _ _)
+                                                       (dsnd a) i f_post c r0));
+      let c' = elim_exists () in
+      assert (PartialMap.equal (PartialMap.upd i (G.reveal c') (repr_to_eht_repr m))
+                               (repr_to_eht_repr (Map.upd m i (G.reveal c'))));
+      rewrite
+        (ETbl.with_key_post_present_predicate _ _ _ _ _ _ _ _)
+        (with_key_post_present_predicate m a i f_post r0 (G.reveal c'));
+
+      intro_exists (G.reveal c') (with_key_post_present_predicate m a i f_post r0);
+
+      rewrite _ (with_key_post m a i f_pre f_post r)
+    | ETbl.Present r0, None ->
+      rewrite
+        (ETbl.with_key_post _ _ _ _ _ _ _)
+        (pure False);
+      elim_pure False;
+      rewrite emp _
+    | ETbl.Absent, _ -> rewrite (ETbl.with_key_post _ _ _ _ _ _ _) _
+    | ETbl.Missing j, _ ->
+      rewrite
+        (ETbl.with_key_post _ _ _ _ _ _ _)
+        (ETbl.tperm (dsnd a) (repr_to_eht_repr m) (PartialMap.empty _ _)
+           `star`
+         f_pre
+           `star`
+         pure (ETbl.map_contains_prop j (repr_to_eht_repr m)));
+      elim_pure _;
+      rewrite
+        (ETbl.tperm (dsnd a) (repr_to_eht_repr m) (PartialMap.empty _ _)
+           `star`
+         f_pre) _
+
+let with_key #k #v #contents #vp #h #m a i #res #f_pre #f_post $f =
+  unpack_perm a;
+  let r = ETbl.with_key (dsnd a) i #_ #f_pre #f_post f in
+  etbl_with_key_post_to_with_key_post a i f_pre f_post r;
+  rewrite _ (with_key_post m a i f_pre f_post r);
+  return r
